Adjust maker tactics to not need arguments
The arguments to the various package making tactics are now carried in
the goal type.  This will make it easier to call the tactics from OCaml.

src/Language/IdentifiersBasicGENERATED.v
@@ -326,8 +326,8 @@ Module Compilers.
   | raw_ident_fancy_addm : raw_ident
   .
 
-  Definition package : GoalType.package.
-  Proof. Tactic.make_package base ident base_type_list_named var_like_idents all_ident_named_interped. Defined.
+  Definition package : GoalType.package_with_args scraped_data var_like_idents base ident.
+  Proof. Tactic.make_package. Defined.
 
   Global Strategy -1000 [base_interp ident_interp].
 End Compilers.
