src/Language/IdentifiersGENERATED.v
@@ -10,8 +10,8 @@ Module Compilers.
     Module ident.
       Export IdentifiersGenerate.Compilers.pattern.ident.
 
-      Definition package : @GoalType.package Compilers.base Compilers.ident.
-      Proof. Time Tactic.make_package IdentifiersBasicGENERATED.Compilers.package IdentifiersBasicGENERATED.Compilers.raw_ident IdentifiersBasicGENERATED.Compilers.pattern_ident. Defined.
+      Definition package : @GoalType.package_with_args Compilers.base Compilers.ident IdentifiersBasicGENERATED.Compilers.package IdentifiersBasicGENERATED.Compilers.raw_ident IdentifiersBasicGENERATED.Compilers.pattern_ident.
+      Proof. Time Tactic.make_package. Defined.
     End ident.
   End pattern.
 End Compilers.
