src/Rewriter/AllTacticsExtra.v
@@ -1,4 +1,5 @@
 Require Import Crypto.Rewriter.AllTactics.
+Require Import Crypto.Rewriter.ProofsCommon.
 Require Import Crypto.Language.IdentifiersBasicGENERATED.
 Require Import Crypto.Language.IdentifiersGENERATEDProofs.
 
@@ -7,14 +8,19 @@ Module Compilers.
   Import Rewriter.AllTactics.Compilers.
 
   Module RewriteRules.
+    Module GoalType.
+      Export ProofsCommon.Compilers.RewriteRules.GoalType.
+      Notation VerifiedRewriter_with_args := (VerifiedRewriter_with_args IdentifiersBasicGENERATED.Compilers.package IdentifiersGENERATEDProofs.Compilers.pattern.ident.package_proofs) (only parsing).
+    End GoalType.
+
     Module Export Tactic.
       Export Rewriter.AllTactics.Compilers.RewriteRules.Tactic.Settings.
 
-      Ltac make_rewriter include_interp specs_proofs :=
-        Rewriter.AllTactics.Compilers.RewriteRules.Tactic.make_rewriter IdentifiersBasicGENERATED.Compilers.package IdentifiersGENERATEDProofs.Compilers.pattern.ident.package_proofs include_interp specs_proofs.
+      Ltac make_rewriter_via include_interp specs_proofs :=
+        Rewriter.AllTactics.Compilers.RewriteRules.Tactic.make_rewriter_via IdentifiersBasicGENERATED.Compilers.package IdentifiersGENERATEDProofs.Compilers.pattern.ident.package_proofs include_interp specs_proofs.
 
-      Tactic Notation "make_rewriter" constr(include_interp) constr(specs_proofs) :=
-        make_rewriter include_interp specs_proofs.
+      Tactic Notation "make_rewriter_via" constr(include_interp) constr(specs_proofs) :=
+        make_rewriter_via include_interp specs_proofs.
     End Tactic.
   End RewriteRules.
 End Compilers.
